

# Brief Introduction to Bernoulli Numbers

Heewon Lee

December 19, 2025

## 1 Introduction: Sum of Powers

Our story begins with the following sum:

$$S_k(n) := 1^k + 2^k + \cdots + n^k = \sum_{i=0}^n i^k.$$

One, of course, could motivate with Gauss' story of adding 1 through 100. Let us take it as an axiom that the reader is interested in these sums. Sometime during high school, we learn the following formulae:

$$S_1(n) = 1 + 2 + \cdots + n = \frac{n(n+1)}{2}$$

$$S_2(n) = 1^2 + 2^2 + \cdots + n^2 = \frac{n(n+1)(2n+1)}{6}$$

$$S_3(n) = 1^3 + 2^3 + \cdots + n^3 = \left( \frac{n(n+1)}{2} \right)^2$$

How do we go forward? If you're lucky, you may have learned an inductive algorithm for the successive formulae using the binomial formula. The following illustrates this for  $S_4(n)$ :

$$\begin{aligned} 1^5 &= 5 \cdot 1^4 - 10 \cdot 1^3 + 10 \cdot 1^2 - 5 \cdot 1^1 + 1 \cdot 1^0 \\ 2^5 - 1^5 &= 5 \cdot 2^4 - 10 \cdot 2^3 + 10 \cdot 2^2 - 5 \cdot 2^1 + 1 \cdot 2^0 \\ 3^5 - 2^5 &= 5 \cdot 3^4 - 10 \cdot 3^3 + 10 \cdot 3^2 - 5 \cdot 3^1 + 1 \cdot 3^0 \\ &\vdots \\ n^5 - (n-1)^5 &= 5 \cdot n^4 - 10 \cdot n^3 + 10 \cdot n^2 - 5 \cdot n^1 + 1 \cdot n^0 \end{aligned}$$

---

$$n^5 = 5S_4(n) - 10S_3(n) + 10S_2(n) - 5S_1(n) + S_0(n)$$

Then, we can solve for  $S_4(n)$  (and recognizing  $S_0(n) = n$ ):

$$\begin{aligned} S_4(n) &= \frac{n^5}{5} + 2S_3(n) - 2S_2(n) + S_1(n) - \frac{1}{5}S_0(n) \\ &= \frac{n^5}{5} + \frac{n^2(n+1)^2}{2} - \frac{n(n+1)(2n+1)}{3} + \frac{n(n+1)}{2} - \frac{n}{5} \\ &= \cdots \\ &= \frac{n^5}{5} + \frac{n^4}{2} + \frac{n^3}{3} - \frac{n}{30}. \end{aligned}$$

This, of course, can be generalized to obtain  $S_k(n)$  for arbitrary  $k$ .

**Theorem 1.1.** *For any  $k \geq 1$ ,  $S_k(n)$  can be expressed as a linear combination of  $S_0(n), S_1(n), \dots, S_{k-1}(n)$  and  $n^{k+1}$ .*

*Proof.* Recall the binomial formula:

$$\begin{aligned}(x-1)^{k+1} &= \sum_{j=0}^{k+1} \binom{k+1}{j} (-1)^{k+1-j} x^j \\ \Rightarrow x^{k+1} - (x-1)^{k+1} &= \sum_{j=0}^k \binom{k+1}{j} (-1)^{k-j} x^j\end{aligned}$$

By taking the sum of both sides from  $x = 1$  to  $x = n$ , the left side telescopes to  $n^{k+1}$  and the right side can be summed termwise:

$$\begin{aligned}n^{k+1} &= \sum_{j=0}^k \binom{k+1}{j} (-1)^{k-j} S_j(n) \\ \Rightarrow S_k(n) &= \frac{n^{k+1}}{k+1} + \frac{1}{k+1} \sum_{j=0}^{k-1} \binom{k+1}{j} (-1)^{k+1-j} S_j(n).\end{aligned}$$

Hence,  $S_k(n)$  is a linear combination of  $S_0(n), S_1(n), \dots, S_{k-1}(n)$  and  $n^{k+1}$ .  $\square$

**Corollary 1.1.1.**  $S_k(n)$  is a polynomial on  $n$  of degree  $k+1$ .

*Proof.* This is justified inductively.  $S_0(n) = n$  is a degree-1 polynomial on  $n$ . If each  $S_l(n)$  is a degree- $(l+1)$  polynomial on  $n$  for every  $l < k$ , then  $S_k(n)$  is a linear combination of  $n^{k+1}$  and polynomials of degrees less than  $k+1$ , where the coefficient of  $n^{k+1}$  is nonzero. Therefore,  $S_k(n)$  is a degree- $(k+1)$  polynomial.  $\square$

Using this algorithm, however, is cumbersome: algebraically solving for  $S_k(n)$  is tedious and error-prone. We need a better method, and fortunately, Corollary 1.1.1 provides one.

## 2 Going Linear

Instead of solving for the function  $S_k(n)$  itself, let us shift the question to calculating their coefficients. Let

$$S_k(n) = a_{k,k}n^{k+1} + a_{k,k-1}n^k + \dots + a_{k,1}n^2 + a_{k,0}n.$$

(Notice the absence of the constant term. This can be justified either inductively or by the fact that  $S_k(0) = 0$ .) We can reformulate this using the following matrix equation:

$$\begin{pmatrix} S_0 \\ S_1 \\ S_2 \\ S_3 \\ \vdots \end{pmatrix} = \begin{pmatrix} a_{00} & 0 & 0 & 0 & \cdots \\ a_{10} & a_{11} & 0 & 0 & \cdots \\ a_{20} & a_{21} & a_{22} & 0 & \cdots \\ a_{30} & a_{31} & a_{32} & a_{33} & \cdots \\ \vdots & \vdots & \vdots & \vdots & \ddots \end{pmatrix} \begin{pmatrix} n^1 \\ n^2 \\ n^3 \\ n^4 \\ \vdots \end{pmatrix}$$

The inductive formula can also be formulated with matrices:

$$\begin{pmatrix} n^1 \\ n^2 \\ n^3 \\ n^4 \\ \vdots \end{pmatrix} = \begin{pmatrix} 1 & 0 & 0 & 0 & \cdots \\ -1 & 2 & 0 & 0 & \cdots \\ 1 & -3 & 3 & 0 & \cdots \\ -1 & 4 & -6 & 4 & \cdots \\ \vdots & \vdots & \vdots & \vdots & \ddots \end{pmatrix} \begin{pmatrix} S_0 \\ S_1 \\ S_2 \\ S_3 \\ \vdots \end{pmatrix}$$

If we chop off at a certain number of rows, then the resulting two coefficient matrices must be inverses of each other. Thus, we are left with the task of computing

$$\begin{pmatrix} a_{00} & 0 & 0 & 0 & \cdots \\ a_{10} & a_{11} & 0 & 0 & \cdots \\ a_{20} & a_{21} & a_{22} & 0 & \cdots \\ a_{30} & a_{31} & a_{32} & a_{33} & \cdots \\ \vdots & \vdots & \vdots & \vdots & \ddots \end{pmatrix} = \begin{pmatrix} 1 & 0 & 0 & 0 & \cdots \\ -1 & 2 & 0 & 0 & \cdots \\ 1 & -3 & 3 & 0 & \cdots \\ -1 & 4 & -6 & 4 & \cdots \\ \vdots & \vdots & \vdots & \vdots & \ddots \end{pmatrix}^{-1}$$

or

$$\begin{pmatrix} 1 & 0 & 0 & 0 & \cdots \\ -1 & 2 & 0 & 0 & \cdots \\ 1 & -3 & 3 & 0 & \cdots \\ -1 & 4 & -6 & 4 & \cdots \\ \vdots & \vdots & \vdots & \vdots & \ddots \end{pmatrix} \begin{pmatrix} a_{00} & 0 & 0 & 0 & \cdots \\ a_{10} & a_{11} & 0 & 0 & \cdots \\ a_{20} & a_{21} & a_{22} & 0 & \cdots \\ a_{30} & a_{31} & a_{32} & a_{33} & \cdots \\ \vdots & \vdots & \vdots & \vdots & \ddots \end{pmatrix} = \begin{pmatrix} 1 & 0 & 0 & 0 & \cdots \\ 0 & 1 & 0 & 0 & \cdots \\ 0 & 0 & 1 & 0 & \cdots \\ 0 & 0 & 0 & 1 & \cdots \\ \vdots & \vdots & \vdots & \vdots & \ddots \end{pmatrix}$$

Directly solving for all  $a_{ij}$  seems hard, so let's try this diagonal by diagonal.

0. Main diagonal:

$$1 = \begin{pmatrix} (-1)^k \binom{k+1}{0} & (-1)^{k-1} \binom{k+1}{1} & \cdots & (-1)^0 \binom{k+1}{k} & 0 & \cdots \end{pmatrix} \cdot \begin{pmatrix} 0 \\ 0 \\ \vdots \\ a_{k,k} \\ a_{k+1,k} \\ \vdots \end{pmatrix} = (k+1)a_{k,k}$$

$$\Rightarrow a_{k,k} = \frac{1}{k+1}$$

1. Subdiagonal:

$$0 = -\binom{k+1}{k-1}a_{k-1,k-1} + \binom{k+1}{k}a_{k,k-1} = -\frac{k(k+1)}{2}\frac{1}{k} + (k+1)a_{k,k-1}$$

$$\Rightarrow a_{k,k-1} = \frac{1}{2}$$

2. Subsubdiagonal:

$$0 = \binom{k+1}{k-2}a_{k-2,k-2} - \binom{k+1}{k-1}a_{k-1,k-2} + \binom{k+1}{k}a_{k,k-2} = \frac{(k+1)k(k-1)}{6}\frac{1}{k-1} - \frac{k(k+1)}{2}\frac{1}{2} + (k+1)a_{k,k-2}$$

$$\Rightarrow a_{k,k-2} = \frac{k}{12}$$

We proceed in this way to obtain:

3.

$$a_{k,k-3} = 0$$

4.

$$a_{k,k-4} = -\frac{k(k-1)(k-2)}{720}$$

5.

$$a_{k,k-5} = 0$$

6.

$$a_{k,k-6} = \frac{k(k-1)(k-2)(k-3)(k-4)}{30240}$$

...

The numerators, in particular, make us form the following ansatz:

**Theorem 2.1.** *We may write*

$$a_{k,k-l} = \frac{B_l}{l!} k(k-1) \cdots (k-l+2) \quad (0 \leq l \leq k),$$

where  $B_l$  are some coefficients and we define the product as  $\frac{1}{k+1}$  for  $l=0$  and 1 for  $l=1$ .

*Proof.* This statement has been proven by brute force for  $l = 0, 1, \dots, 6$ . We proceed inductively, using the  $l$ th subdiagonal in our matrix equation:

$$\begin{aligned}
0 &= (-1)^l \binom{k+1}{k-l} a_{k-l, k-l} + (-1)^{l-1} \binom{k+1}{k-l+1} a_{k-l+1, k-l} + \dots + (-1)^0 \binom{k+1}{k} a_{k, k-l} \\
\Rightarrow a_{k, k-l} &= \frac{k}{2!} a_{k-1, k-l} - \frac{k(k-1)}{3!} a_{k-2, k-l} + \dots + (-1)^{l+1} \frac{k(k-1) \dots (k-l+1)}{(l+1)!} a_{k-l, k-l} \\
&= \sum_{j=1}^l (-1)^{j+1} \frac{\prod_{i=0}^{j-1} (k-i)}{(j+1)!} \cdot a_{k-j, k-l} \\
&= \sum_{j=1}^l (-1)^{j+1} \frac{\prod_{i=0}^{j-1} (k-i)}{(j+1)!} \cdot \frac{B_{l-j}}{(l-j)!} \prod_{i=0}^{l-j-2} (k-j-i) \\
&= \left( \frac{1}{l+1} \sum_{j=1}^l (-1)^{j+1} \binom{l+1}{j+1} B_{l-j} \right) \cdot \frac{k(k-1) \dots (k-l+2)}{l!}
\end{aligned}$$

Therefore, the formula holds for all  $l$ . □

**Corollary 2.1.1.** For any  $l$ ,

$$\sum_{j=0}^l (-1)^j \binom{l+1}{j+1} B_{l-j} = \delta_{l0},$$

where  $\delta_{l0}$  is the Kronecker delta, equal to 1 if  $l = 0$  and 0 otherwise.

*Proof.* For  $l > 0$ , the above formula

$$B_l = \frac{1}{l+1} \sum_{j=1}^l (-1)^{j+1} \binom{l+1}{j+1} B_{l-j}$$

is equivalent to this theorem. For  $l = 0$ , the left-hand side is  $B_0$ , which is equal to 0. □

We now have an algorithm for calculating arbitrary sums of powers!

1. Calculate sufficiently many  $B_n$ 's, using Corollary 2.1.1.
2.  $a_{k, k-j} = \frac{B_j}{j!} k(k-1) \dots (k-j+2)$
3.  $S_k(n) = a_{k, k} n^{k+1} + a_{k, k-1} n^k + \dots + a_{k, 0} n^1$

As an example, let us calculate  $S_{10}(10)$ .

$$\{B_n\} = 1, \frac{1}{2}, \frac{1}{6}, 0, -\frac{1}{30}, 0, \frac{1}{42}, 0, -\frac{1}{30}, 0, \frac{5}{66}, \dots$$

(Why so many zeros? Stay tuned...)

$$\Rightarrow a_{10, 10} = \frac{1}{11}, a_{10, 9} = \frac{1}{2}, a_{10, 8} = \frac{5}{6}, a_{10, 7} = 0, a_{10, 6} = -1, a_{10, 5} = 0, a_{10, 4} = 1,$$

$$a_{10, 3} = 0, a_{10, 2} = -\frac{1}{2}, a_{10, 1} = 0, a_{10, 0} = \frac{5}{66}$$

$$\begin{aligned}
1^{10} + 2^{10} + \dots + 10^{10} &= \frac{10^{11}}{11} + \frac{10^{10}}{2} + \frac{5}{6} 10^9 - 10^7 + 10^5 - \frac{10^3}{2} + \frac{5}{66} 10^1 \\
&= 10 \left( \frac{5}{66} + 100 \left( -\frac{1}{2} + 100 \left( 1 + 100 \left( \frac{5}{6} + 10 \left( \frac{1}{2} + \frac{10}{11} \right) \right) \right) \right) \right) \\
&= 14914341925
\end{aligned}$$

This was barely less effort than directly summing the expression!

### 3 Bernoulli Numbers

The numbers  $B_n$  we have defined are the infamous *Bernoulli numbers*, and the power sum formulae we found are called *Faulhaber's formula*. Explicitly, this is:

$$S_k(n) = 1^k + 2^k + \cdots + n^k = \frac{1}{k+1} \sum_{j=1}^{k+1} \binom{k+1}{j} B_{k+1-j} n^j.$$

When analyzing any sequence, one overpowered tool is its generating function. Consider the following:

$$f(x) := \sum_{n=0}^{\infty} \frac{B_n}{n!} x^n.$$

(Let us postpone the question of convergence for later, which is standard procedure.) Let us use the inductive formula from Corollary 2.1.1 again:

$$\delta_{l0} = \sum_{j=0}^l (-1)^j \binom{l+1}{j+1} B_{l-j} = (l+1)! \sum_{j=0}^l \frac{(-1)^j}{(j+1)! (l-j)!} B_{l-j}.$$

The last expression could very well arise from a product of  $f(x)$  and

$$\begin{aligned} \sum_{n=0}^{\infty} \frac{(-1)^n}{(n+1)!} x^{n+1} &= -\frac{1}{x} \sum_{n=0}^{\infty} \frac{(-1)^{n+1}}{(n+1)!} x^{n+1} = \frac{1 - e^{-x}}{x}. \\ \Rightarrow \frac{1 - e^{-x}}{x} f(x) &= \sum_{n=0}^{\infty} x^n \sum_{j=0}^n \frac{(-1)^j}{(j+1)! (n-j)!} B_{n-j} = \sum_{n=0}^{\infty} x^n \delta_{n0} = 1 \\ \therefore f(x) &= \sum_{n=0}^{\infty} \frac{B_n}{n!} x^n = \frac{x}{1 - e^{-x}} \end{aligned}$$

We thus obtain the closed-form expression

$$B_n = \left. \frac{d^n}{dx^n} \left( \frac{x}{1 - e^{-x}} \right) \right|_{x=0}$$

or using Cauchy's integral formula,

$$B_n = \frac{n!}{2\pi i} \oint_{|z|=1} \frac{dz}{z^n (1 - e^{-z})}$$

with the contour oriented counterclockwise around the origin. Returning to the question of convergence, notice that the poles of the complex function  $f(z)$  are precisely  $z = \pm i n \pi$  for positive integers  $n$ . The closest poles to the origin are  $\pm i \pi$ ; therefore, the series converges when  $|z| < \pi$ . The convergence for when  $|z| = \pi$  is left as an exercise.

**Theorem 3.1.** For  $n > 1$  odd,  $B_n = 0$ .

*Proof.* Notice that

$$\begin{aligned} f(x) - f(-x) &= \sum_{n=0}^{\infty} \frac{B_n}{n!} (x^n - (-x)^n) = \sum_{n \text{ odd}} \frac{2B_n}{n!} x^n \\ &= \frac{x}{1 - e^{-x}} - \frac{-x}{1 - e^x} = \frac{x(1 - e^{-x})}{1 - e^{-x}} = x. \end{aligned}$$

Therefore,  $B_n = 0$  for all odd  $n > 1$ . □

### 4 Euler-Maclaurin Formula

TODO